Add more comments and rewrote some proofs in PFunc.v

src/PFunc.v
@@ -5,17 +5,40 @@ Local Open Scope Z_scope.
 
 Local Set Warnings "-notation-overridden".
 
+(* V represent either an element in Z, no element, or all values in Z *)
 Inductive V :=
 | VTop
 | VVal (n: Z)
 | VBot.
 
-Definition eq_V (v1 v2: V) :=
+Definition eqV (v1 v2: V) :=
   match (v1, v2) with
   | (VTop, VTop) => true
   | (VBot, VBot) => true
   | (VVal v1, VVal v2) => v1 == v2
   | _ => false
+  end.
+
+Lemma eqVP : Equality.axiom eqV.
+Proof.
+  case => [ | z1 | ]; case => [ | z2 | ]; apply (iffP idP) => //.
+  - by rewrite /eqV => /eqP ->.
+  - rewrite /eqV => [[->]].
+      by auto.
+Qed.
+
+(* Canonical structure for V with ewuality *)
+
+Canonical V_eqMixin := EqMixin eqVP.
+Canonical V_eqType := Eval hnf in EqType V V_eqMixin.
+
+(* Some useful definitions and proofs dealing with V *)
+
+Definition in_V (n: Z) (v: V) :=
+  match v with
+  | VTop => true
+  | VVal n' => n == n'
+  | VBot => false
   end.
 
 Definition le_V (v1 v2: V) :=
@@ -25,11 +48,12 @@ Definition le_V (v1 v2: V) :=
   | (VVal n1, VVal n2) => n1 == n2
   | _ => false
   end.
+Hint Unfold le_V.
 
 Theorem le_V_refl : forall v, (le_V v v).
 Proof.
   case => // n.
-  by apply Z.eqb_refl.
+  by apply eq_refl.
 Qed.
 
 Theorem le_V_trans :
@@ -37,42 +61,27 @@ Theorem le_V_trans :
 Proof.
   move => v1 v2 v3.
   case v1; case v2; case v3 => //.
-  rewrite /le_V.
-  move => n3 n2 n1 /Z.eqb_spec H12 /Z.eqb_spec H23.
+  rewrite /le_V => n3 n2 n1 /eqP H12 /eqP H23.
   rewrite H12 H23.
-    by apply /Z.eqb_spec.
+    by apply /eqP.
 Qed.
-
-Definition in_V (n: Z) (v: V) :=
-  match v with
-  | VTop => true
-  | VVal n' => n == n'
-  | VBot => false
-  end.
 
 Definition le_V_spec :
   forall v1 v2, le_V v1 v2 <-> forall n, in_V n v1 -> in_V n v2.
 Proof.
   move => v1 v2.
-  split.
-  - case v1; case v2 => // n n0.
-    rewrite /le_V => /Z.eqb_spec -> //.
-  - case v1; case v2 => //.
-    + move => n /= /(_ (n+1) is_true_true) /eqP Himpossible.
+  split. by case v1; case v2 => // n n0; rewrite /le_V => /eqP -> //.
+  case v1; case v2 => //.
+  - move => n /= /(_ (n+1) is_true_true) /eqP Himpossible.
       by apply Z.neq_succ_diag_l in Himpossible.
-    + move => Hle.
-        by have /Hle : (in_V 0 VTop) by [] => Himpossible.
-    + move => n n0 Hin.
-      case (Z.eqb_spec n n0).
-      * move => Heq.
-          by rewrite Heq /le_V.
-      * move => /Z.eqb_spec Hne.
-        move: (Hin n0) => Himpossible.
-        have /Himpossible : (in_V n0 (VVal n0)); by rewrite /in_V.
-    + move => n Hin.
-      move: (Hin n) => Hin'.
-      have /Hin' : (in_V n (VVal n)). by rewrite /in_V.
-        by move => Himpossible.
+  - move => /= /(_ 0).
+      by auto.
+  - move => n n0 Hin.
+    case (n =P n0) => [ -> | ].
+    + by rewrite /le_V.
+    + move => /eqP Hne.
+      by move: (Hin n0) => /= /(_ (eq_refl n0)) Himpossible.
+  - by move => n /(_ n (eq_refl n)) Hin.
 Qed.
 
 Definition binop_V (v1 v2: V) (op: Z -> Z -> Z):=
@@ -82,7 +91,7 @@ Definition binop_V (v1 v2: V) (op: Z -> Z -> Z):=
   | (VVal v1, VVal v2) => VVal (op v1 v2)
   end.
 
-Definition add_V (v1 v2: V) :=
+Definition add_V v1 v2 :=
   binop_V v1 v2 Z.add.
 
 Theorem add_V_spec :
@@ -91,13 +100,11 @@ Theorem add_V_spec :
                     in_V (x1 + x2) (add_V v1 v2).
 Proof.
   move => x1 v1 H1 x2 v2 H2.
-  rewrite /in_V /add_V /binop_V.
-  case v1 eqn:Hv1; case v2 eqn:Hv2 => //.
-  rewrite /= in H1 H2.
-  by move: H1 H2 => /eqP -> /eqP ->.
+  rewrite /in_V /binop_V.
+  by case: v1 H1 H2; case v2 => //= n n0 /eqP -> /eqP ->.
 Qed.
 
-Definition sub_V (v1 v2: V) :=
+Definition sub_V v1 v2 :=
   binop_V v1 v2 Z.sub.
 
 Theorem sub_V_spec :
@@ -106,10 +113,8 @@ Theorem sub_V_spec :
                     in_V (x1 - x2) (sub_V v1 v2).
 Proof.
   move => x1 v1 H1 x2 v2 H2.
-  rewrite /in_V /sub_V /binop_V.
-  case v1 eqn:Hv1; case v2 eqn:Hv2 => //.
-  rewrite /= in H1 H2.
-  by move: H1 H2 => /eqP -> /eqP ->.
+  rewrite /in_V /binop_V.
+  by case: v1 H1 H2; case v2 => //= n n0 /eqP -> /eqP ->.
 Qed.
 
 Definition le_binop_V (v1 v2: V) :=
@@ -122,9 +127,7 @@ Theorem le_binop_V_spec :
 Proof.
   move => x1 v1 H1 x2 v2 H2.
   rewrite /in_V /le_binop_V /binop_V.
-  case v1 eqn:Hv1; case v2 eqn:Hv2 => //.
-  rewrite /= in H1 H2.
-  by move: H1 H2 => /eqP -> /eqP ->.
+  by case: v1 H1 H2; case v2 => //= n n0 /eqP -> /eqP ->.
 Qed.
 
 Definition unop_V (v: V) (op: Z -> Z) :=
@@ -135,6 +138,10 @@ Definition unop_V (v: V) (op: Z -> Z) :=
 
 Definition mul_V (z: Z) (v: V) :=
   unop_V v (fun v => z * v).
+
+Hint Resolve le_V_refl add_V_spec sub_V_spec le_binop_V_spec.
+
+(* Specification of a PFunc *)
 
 Class PFuncImpl (PFunc: Type) :=
   {
@@ -186,18 +193,20 @@ Class PFuncImpl (PFunc: Type) :=
     pfunc_restrict_ne_set: PFunc -> Z -> PFunc;
     pfunc_restrict_ne_set_spec:
       forall p m v, eval_pfunc (pfunc_restrict_ne_set p v) m =
-               if eq_V (eval_pfunc p m) (VVal v) then
+               if (eval_pfunc p m) == (VVal v) then
                  VBot
                else
                  (eval_pfunc p m);
   }.
+
+Hint Resolve le_pfunc_spec join_pfunc_spec_l join_pfunc_spec_r.
 
 Theorem le_pfunc_refl {PFunc: Type} {PI: PFuncImpl PFunc} :
   forall a, le_pfunc a a.
 Proof.
   move => a.
   apply le_pfunc_spec => x.
-  apply le_V_refl.
+  by auto.
 Qed.
 
 Theorem le_pfunc_trans {PFunc: Type} {PI: PFuncImpl PFunc} :
@@ -205,7 +214,7 @@ Theorem le_pfunc_trans {PFunc: Type} {PI: PFuncImpl PFunc} :
 Proof.
   move => a1 a2 a3 /le_pfunc_spec H12 /le_pfunc_spec H23.
   apply le_pfunc_spec => x.
-    by apply (le_V_trans _ (eval_pfunc a2 x)).
+  by eapply le_V_trans.
 Qed.
 
 Theorem is_constant_on_var_update_spec {PFunc: Type} {PI: PFuncImpl PFunc} :
@@ -213,11 +222,9 @@ Theorem is_constant_on_var_update_spec {PFunc: Type} {PI: PFuncImpl PFunc} :
              forall z m, eval_pfunc p (v !-> z; m) = eval_pfunc p m.
 Proof.
   move => p v Hconst z m.
-  apply (iffLR (is_constant_on_var_spec _ _)) with
-        (m0 := eval_map m)
-        (m' := eval_map (v !-> z; m))
-      in Hconst => [ // | v' Hne ].
-    by simpl_totalmap.
+  eapply is_constant_on_var_spec; eauto.
+  move => v' Hne.
+  by simpl_totalmap.
 Qed.
 
 (* A useful lemma used in the next tactic *)
@@ -229,6 +236,7 @@ Proof.
     by simpl_totalmap.
 Qed.
 
+(* Useful tactic to simplify goal when using pfunc *)
 
 Ltac simpl_pfunc :=
   repeat match goal with
